proof-libs/coq/coq/generated-core/src/Core_Slice.v
@@ -12,57 +12,16 @@ Import RecordSetNotations.
 
 (* From Core Require Import Core. *)
 
-(* TODO: Replace this dummy lib with core lib *)
-Class t_Sized (T : Type) := { }.
-Definition t_u8 := Z.
-Definition t_u16 := Z.
-Definition t_u32 := Z.
-Definition t_u64 := Z.
-Definition t_u128 := Z.
-Definition t_usize := Z.
-Definition t_i8 := Z.
-Definition t_i16 := Z.
-Definition t_i32 := Z.
-Definition t_i64 := Z.
-Definition t_i128 := Z.
-Definition t_isize := Z.
-Definition t_Array T (x : t_usize) := list T.
-Definition t_String := string.
-Definition ToString_f_to_string (x : string) := x.
-Instance Sized_any : forall {t_A}, t_Sized t_A := {}.
-Class t_Clone (T : Type) := { Clone_f_clone : T -> T }.
-Instance Clone_any : forall {t_A}, t_Clone t_A := {Clone_f_clone := fun x => x}.
-Definition t_Slice (T : Type) := list T.
-Definition unsize {T : Type} : list T -> t_Slice T := id.
-Definition t_PartialEq_f_eq x y := x =? y.
-Definition t_Rem_f_rem (x y : Z) := x mod y.
-Definition assert (b : bool) (* `{H_assert : b = true} *) : unit := tt.
-Inductive globality := | t_Global.
-Definition t_Vec T (_ : globality) : Type := list T.
-Definition impl_1__append {T} l1 l2 : list T * list T := (app l1 l2, l2).
-Definition impl_1__len {A} (l : list A) := Z.of_nat (List.length l).
-Definition impl__new {A} (_ : Datatypes.unit) : list A := nil.
-Definition impl__with_capacity {A} (_ : Z)  : list A := nil.
-Definition impl_1__push {A} l (x : A) := cons x l.
-Class t_From (A B : Type) := { From_f_from : B -> A }.
-Definition impl__to_vec {T} (x : t_Slice T) : t_Vec T t_Global := x.
-Class t_Into (A B : Type) := { Into_f_into : A -> B }.
-Instance t_Into_from_t_From {A B : Type} `{H : t_From B A} : t_Into A B := { Into_f_into x := @From_f_from B A H x }.
-Definition from_elem {A} (x : A) (l : Z) := repeat x (Z.to_nat l).
-Definition t_Option := option.
-Definition impl__map {A B} (x : t_Option A) (f : A -> B) : t_Option B := match x with | Some x => Some (f x) | None => None end.
-Definition t_Add_f_add x y := x + y.
-Class Cast A B := { cast : A -> B }.
-Instance cast_t_u8_t_u32 : Cast t_u8 t_u32 := {| cast x := x |}.
-(* / dummy lib *)
-
-From Core Require Import Core_Primitive (t_Slice).
-Export Core_Primitive (t_Slice).
+From Core Require Import Core_Primitive.
+Export Core_Primitive.
 
 
 
-From Core Require Import Iter (t_Iter).
-Export Iter (t_Iter).
+From Core Require Import Core_Slice_Iter.
+Export Core_Slice_Iter.
+
+From Core Require Import Core_Convert.
+Export Core_Convert.
 
 (* NotImplementedYet *)
 
@@ -75,4 +34,4 @@ Definition impl__len `{v_T : Type} `{t_Sized (v_T)} `{t_Clone (v_T)} (self : t_S
   From_f_from (len (Clone_f_clone (Slice_f_v self))).
 
 Definition impl__is_empty `{v_T : Type} `{t_Sized (v_T)} `{t_Clone (v_T)} (self : t_Slice ((v_T))) : bool :=
-  t_PartialEq_f_eq (impl__len (self)) (0).
+  PartialEq_f_eq (impl__len (self)) (Build_t_usize (Build_t_U64 0%N)).
