proof-libs/coq/coq/generated-core/src/Core.v
@@ -64,6 +64,15 @@ Export Core_Primitive.
 From Core Require Import Core_Option.
 Export Core_Option.
 
+From Core Require Import Core_Array_Rec_bundle_579704328.
+Export Core_Array_Rec_bundle_579704328.
+
+From Core Require Import Core_Ops.
+Export Core_Ops.
+
+From Core Require Import Core_Ops_Index.
+Export Core_Ops_Index.
+
 From Core Require Import NumberNotation.
 Export NumberNotation.
 
