proof-libs/coq/coq/generated-core/src/Core_Ops_Index_range.v
@@ -15,8 +15,8 @@ Import RecordSetNotations.
 From Core Require Import Core_Primitive.
 Export Core_Primitive.
 
-From Core Require Import Core_Iter (t_Iterator).
-Export Core_Iter (t_Iterator).
+From Core Require Import Core_Iter_Traits_Iterator.
+Export Core_Iter_Traits_Iterator.
 
 Record t_IndexRange : Type :=
   {
@@ -30,32 +30,34 @@ Arguments IndexRange_f_end.
   settable! (Build_t_IndexRange) <IndexRange_f_start; IndexRange_f_end>.
 
 Definition impl__IndexRange__zero_to (v_end : t_usize) : t_IndexRange :=
-  Build_t_IndexRange (0) (v_end).
+  Build_t_IndexRange (Build_t_usize (Build_t_U64 0%N)) (v_end).
 
 Definition impl__IndexRange__next_unchecked (self : t_IndexRange) : (t_IndexRange*t_usize) :=
   let value := IndexRange_f_start self in
-  let self := self <|IndexRange_f_start := t_Add_f_add (value) (1) |> in
+  let self := self <|IndexRange_f_start := Add_f_add (value) (Build_t_usize (Build_t_U64 1%N) : t_usize) |> in
   let hax_temp_output := value in
   (self,hax_temp_output).
 
 Definition impl__IndexRange__len (self : t_IndexRange) : t_usize :=
-  sub (IndexRange_f_end self) (IndexRange_f_start self).
+  Sub_f_sub (IndexRange_f_end self) (IndexRange_f_start self).
 
-Instance t_Iterator_538767852 : t_Iterator ((t_IndexRange)) :=
+Program Instance t_Iterator_538767852 : t_Iterator ((t_IndexRange)) :=
   {
-    Iterator_impl_1_f_Item := t_usize;
-    Iterator_impl_1_f_next := fun  (self : t_IndexRange)=>
-      let hax_temp_output := never_to_any (panic_fmt (impl_2__new_v1 (["not yet implemented: specification needed"%string]) (impl_1__none (tt)))) in
-      (self,hax_temp_output);
-    Iterator_impl_1_f_size_hint := fun  (self : t_IndexRange)=>
+    Iterator_f_Item := t_usize;
+    Iterator_f_next := fun  (self : t_IndexRange)=>
+      (* let hax_temp_output := never_to_any (panic ("not yet implemented: specification needed"%string)) in *)
+      (self,Option_Some (self.(IndexRange_f_start)));
+    Iterator_f_size_hint := fun  (self : t_IndexRange)=>
       let len := impl__IndexRange__len (self) in
       (len,Option_Some (len));
-    Iterator_impl_1_f_fold := fun  (self : t_IndexRange) (init : v_B) (f : v_F)=>
-      never_to_any (panic_fmt (impl_2__new_v1 (["not yet implemented: specification needed"%string]) (impl_1__none (tt))));
+    Iterator_f_fold := fun {v_B : Type} {v_F : Type} `{t_Sized v_B} `{t_Sized v_F} `{t_Sized t_IndexRange} (_ : t_FnOnce v_F (v_B * t_usize)) (_ : t_FnMut v_F (v_B * t_usize)) `{_ : FnOnce_f_Output = v_B} (self : t_IndexRange) (init : v_B) (f : v_F)=>
+      never_to_any (panic "not yet implemented: specification needed"%string);
   }.
+Next Obligation.
+Admitted.
 
-Instance t_ExactSizeIterator_661616782 : t_ExactSizeIterator ((t_IndexRange)) :=
-  {
-    ExactSizeIterator_impl_2_f_len := fun  (self : t_IndexRange)=>
-      impl__IndexRange__len (self);
-  }.
+(* Instance t_ExactSizeIterator_661616782 : t_ExactSizeIterator ((t_IndexRange)) := *)
+(*   { *)
+(*     ExactSizeIterator_impl_2_f_len := fun  (self : t_IndexRange)=> *)
+(*       impl__IndexRange__len (self); *)
+(*   }. *)
